preservation tmp

theories/opsem.v
@@ -24,44 +24,54 @@ Inductive reduce_simple : seq administrative_instruction -> seq administrative_i
 
 (** unop **)
   | rs_unop : forall v op t,
-    reduce_simple [::$VA v; AI_basic (BI_unop t op)] [::$VA (@app_unop op v)]
+    reduce_simple [::$VN v; AI_basic (BI_unop t op)] [::$VN (@app_unop op v)]
                    
 (** binop **)
   | rs_binop_success : forall v1 v2 v op t,
     app_binop op v1 v2 = Some v ->
-    reduce_simple [::$VA v1; $VA v2; AI_basic (BI_binop t op)] [::$VA v]
+    reduce_simple [::$VN v1; $VN v2; AI_basic (BI_binop t op)] [::$VN v]
   | rs_binop_failure : forall v1 v2 op t,
     app_binop op v1 v2 = None ->
-    reduce_simple [::$VA v1; $VA v2; AI_basic (BI_binop t op)] [::AI_trap]
+    reduce_simple [::$VN v1; $VN v2; AI_basic (BI_binop t op)] [::AI_trap]
                   
   (** testops **)
   | rs_testop_i32 :
     forall c testop,
-    reduce_simple [::$VA (VAL_int32 c); AI_basic (BI_testop T_i32 testop)] [::$VA (VAL_int32 (wasm_bool (@app_testop_i i32t testop c)))]
+    reduce_simple [::$VN (VAL_int32 c); AI_basic (BI_testop T_i32 testop)] [::$VN (VAL_int32 (wasm_bool (@app_testop_i i32t testop c)))]
   | rs_testop_i64 :
     forall c testop,
-    reduce_simple [::$VA (VAL_int64 c); AI_basic (BI_testop T_i64 testop)] [::$VA (VAL_int32 (wasm_bool (@app_testop_i i64t testop c)))]
+    reduce_simple [::$VN (VAL_int64 c); AI_basic (BI_testop T_i64 testop)] [::$VN (VAL_int32 (wasm_bool (@app_testop_i i64t testop c)))]
 
   (** relops **)
   | rs_relop: forall v1 v2 t op,
-    reduce_simple [::$VA v1; $VA v2; AI_basic (BI_relop t op)] [::$VA (VAL_int32 (wasm_bool (app_relop op v1 v2)))]
+    reduce_simple [::$VN v1; $VN v2; AI_basic (BI_relop t op)] [::$VN (VAL_int32 (wasm_bool (app_relop op v1 v2)))]
                     
   (** convert and reinterpret **)
   | rs_convert_success :
     forall t1 t2 v v' sx,
     types_agree (T_num t1) (VAL_num v) ->
     cvt t2 sx v = Some v' ->
-    reduce_simple [::$VA v; AI_basic (BI_cvtop t2 CVO_convert t1 sx)] [::$VA v']
+    reduce_simple [::$VN v; AI_basic (BI_cvtop t2 CVO_convert t1 sx)] [::$VN v']
   | rs_convert_failure :
     forall t1 t2 v sx,
     types_agree (T_num t1) (VAL_num v) ->
     cvt t2 sx v = None ->
-    reduce_simple [::$VA v; AI_basic (BI_cvtop t2 CVO_convert t1 sx)] [::AI_trap]
+    reduce_simple [::$VN v; AI_basic (BI_cvtop t2 CVO_convert t1 sx)] [::AI_trap]
   | rs_reinterpret :
     forall t1 t2 v,
     types_agree (T_num t1) (VAL_num v) ->
-    reduce_simple [::$VA v; AI_basic (BI_cvtop t2 CVO_reinterpret t1 None)] [::$VA (wasm_deserialise (bits v) t2)]
+    reduce_simple [::$VN v; AI_basic (BI_cvtop t2 CVO_reinterpret t1 None)] [::$VN (wasm_deserialise (bits v) t2)]
 
+  (** reference operations **)
+  | rs_ref_is_null_true:
+    forall t,
+    reduce_simple [:: $V (VAL_ref (VAL_ref_null t)); AI_basic BI_ref_is_null] [::$VN (VAL_int32 Wasm_int.Int32.one)]
+  (* This formulation might cause some difficulty in the proofs, but it's the most faithful to the spec *)
+  | rs_ref_is_null_false:
+    forall ref,
+    (forall t, ref <> VAL_ref_null t) ->
+    reduce_simple [:: $V (VAL_ref ref); AI_basic BI_ref_is_null] [::$VN (VAL_int32 Wasm_int.Int32.zero)]
+                  
   (** control-flow operations **)
   | rs_unreachable :
     reduce_simple [::AI_basic BI_unreachable] [::AI_trap]
@@ -69,15 +79,15 @@ Inductive reduce_simple : seq administrative_instruction -> seq administrative_i
     reduce_simple [::AI_basic BI_nop] [::]
   | rs_drop :
     forall v,
-    reduce_simple [::$VA v; AI_basic BI_drop] [::]
+    reduce_simple [::$V v; AI_basic BI_drop] [::]
   | rs_select_false :
     forall n v1 v2 ot,
     n = Wasm_int.int_zero i32m ->
-    reduce_simple [::$VA v1; $VA v2; $VA (VAL_int32 n); AI_basic (BI_select ot)] [::$VA v2]
+    reduce_simple [::$V v1; $V v2; $VN (VAL_int32 n); AI_basic (BI_select ot)] [::$V v2]
   | rs_select_true :
     forall n v1 v2 ot,
     n <> Wasm_int.int_zero i32m ->
-    reduce_simple [::$VA v1; $VA v2; $VA (VAL_int32 n); AI_basic (BI_select ot)] [::$VA v1]
+    reduce_simple [::$V v1; $V v2; $VN (VAL_int32 n); AI_basic (BI_select ot)] [::$V v1]
   | rs_label_const :
       forall n es vs,
         const_list vs ->
@@ -85,6 +95,14 @@ Inductive reduce_simple : seq administrative_instruction -> seq administrative_i
   | rs_label_trap :
       forall n es,
         reduce_simple [::AI_label n es [::AI_trap]] [::AI_trap]
+  | rs_if_false :
+    forall c tb es1 es2,
+      c = Wasm_int.int_zero i32m ->
+      reduce_simple ([::$VN (VAL_int32 c); AI_basic (BI_if tb es1 es2)]) [::AI_basic (BI_block tb es2)]
+  | rs_if_true :
+    forall c tb es1 es2,
+      c <> Wasm_int.int_zero i32m ->
+      reduce_simple ([::$VN (VAL_int32 c); AI_basic (BI_if tb es1 es2)]) [::AI_basic (BI_block tb es1)]
   | rs_br :
       forall n vs es i LI (lh: lholed i),
         const_list vs ->
@@ -94,20 +112,20 @@ Inductive reduce_simple : seq administrative_instruction -> seq administrative_i
   | rs_br_if_false :
       forall n i,
         n = Wasm_int.int_zero i32m ->
-        reduce_simple [::$VA (VAL_int32 n); AI_basic (BI_br_if i)] [::]
+        reduce_simple [::$VN (VAL_int32 n); AI_basic (BI_br_if i)] [::]
   | rs_br_if_true :
       forall n i,
         n <> Wasm_int.int_zero i32m ->
-        reduce_simple [::$VA (VAL_int32 n); AI_basic (BI_br_if i)] [::AI_basic (BI_br i)]
+        reduce_simple [::$VN (VAL_int32 n); AI_basic (BI_br_if i)] [::AI_basic (BI_br i)]
   | rs_br_table :
       forall iss c i j,
         length iss > Wasm_int.nat_of_uint i32m c ->
         List.nth_error iss (Wasm_int.nat_of_uint i32m c) = Some j ->
-        reduce_simple [::$VA (VAL_int32 c); AI_basic (BI_br_table iss i)] [::AI_basic (BI_br j)]
+        reduce_simple [::$VN (VAL_int32 c); AI_basic (BI_br_table iss i)] [::AI_basic (BI_br j)]
   | rs_br_table_length :
       forall iss c i,
         length iss <= (Wasm_int.nat_of_uint i32m c) ->
-        reduce_simple [::$VA (VAL_int32 c); AI_basic (BI_br_table iss i)] [::AI_basic (BI_br i)]
+        reduce_simple [::$VN (VAL_int32 c); AI_basic (BI_br_table iss i)] [::AI_basic (BI_br i)]
   | rs_local_const :
       forall es n f,
         const_list es ->
@@ -116,16 +134,15 @@ Inductive reduce_simple : seq administrative_instruction -> seq administrative_i
   | rs_local_trap :
       forall n f,
         reduce_simple [::AI_frame n f [::AI_trap]] [::AI_trap]
+  | rs_local_tee :
+      forall i v,
+        reduce_simple [::$V v; AI_basic (BI_local_tee i)] [::$V v; $V v; AI_basic (BI_local_set i)]
   | rs_return :
       forall n i vs es (lh: lholed i) f,
         const_list vs ->
         length vs = n ->
         lfill lh (vs ++ [::AI_basic BI_return]) = es ->
         reduce_simple [::AI_frame n f es] vs
-  | rs_tee_local :
-      forall i v,
-        is_const v ->
-        reduce_simple [::v; AI_basic (BI_local_tee i)] [::v; v; AI_basic (BI_local_set i)]
   | rs_trap :
       forall es (lh: lholed 0),
         es <> [::AI_trap] ->
@@ -139,6 +156,10 @@ Inductive reduce : host_state -> store_record -> frame -> list administrative_in
       forall e e' s f hs,
         reduce_simple e e' ->
         reduce hs s f e hs s f e'
+  | r_ref_func:
+    forall hs s f addr x,
+      lookup_N f.(f_inst).(inst_funcs) x = Some addr ->
+      reduce hs s f [::AI_basic (BI_ref_func x)] hs s f [::AI_ref addr]
   | r_block :
     forall hs s f vs es n m tb t1s t2s,
       expand f.(f_inst) tb = Some (Tf t1s t2s) ->
@@ -147,7 +168,7 @@ Inductive reduce : host_state -> store_record -> frame -> list administrative_in
       length t1s = n ->
       length t2s = m ->
       reduce hs s f (vs ++ [::AI_basic (BI_block tb es)]) hs s f [::AI_label m [::] (vs ++ to_e_list es)]
-  | rs_loop :
+  | r_loop :
       forall hs s f vs es n m tb t1s t2s,
       expand f.(f_inst) tb = Some (Tf t1s t2s) ->
       const_list vs ->
@@ -155,24 +176,6 @@ Inductive reduce : host_state -> store_record -> frame -> list administrative_in
       length t1s = n ->
       length t2s = m ->
       reduce hs s f (vs ++ [::AI_basic (BI_loop tb es)]) hs s f [::AI_label n [::AI_basic (BI_loop tb es)] (vs ++ to_e_list es)]
-  | rs_if_false :
-    forall hs s f c vs es1 es2 n m tb t1s t2s,
-      expand f.(f_inst) tb = Some (Tf t1s t2s) ->
-      c = Wasm_int.int_zero i32m ->
-      const_list vs ->
-      length vs = m ->
-      length t1s = m ->
-      length t2s = n ->
-      reduce hs s f (vs ++ [::$VA (VAL_int32 c); AI_basic (BI_if tb es1 es2)]) hs s f [::AI_label n [::] (vs ++ to_e_list es2)]
-  | rs_if_true :
-    forall hs s f c vs es1 es2 n m tb t1s t2s,
-      expand f.(f_inst) tb = Some (Tf t1s t2s) ->
-      c <> Wasm_int.int_zero i32m ->
-      const_list vs ->
-      length vs = m ->
-      length t1s = m ->
-      length t2s = n ->
-      reduce hs s f (vs ++ [::$VA (VAL_int32 c); AI_basic (BI_if tb es1 es2)]) hs s f [::AI_label n [::] (vs ++ to_e_list es1)]
   (** calling operations **)
   | r_call :
       forall s f (i: funcidx) a hs,
@@ -183,26 +186,26 @@ Inductive reduce : host_state -> store_record -> frame -> list administrative_in
         stab_elem s f.(f_inst) x (Wasm_int.N_of_uint i32m i) = Some (VAL_ref_func a) ->
         List.nth_error s.(s_funcs) a = Some cl ->
         List.nth_error f.(f_inst).(inst_types) y = Some (cl_type cl) ->
-        reduce hs s f [::$VA (VAL_int32 i); AI_basic (BI_call_indirect x y)] hs s f [::AI_invoke a]
+        reduce hs s f [::$VN (VAL_int32 i); AI_basic (BI_call_indirect x y)] hs s f [::AI_invoke a]
   | r_call_indirect_failure1 :
       forall s f x (y: typeidx) a cl i hs,
         stab_elem s f.(f_inst) x (Wasm_int.N_of_uint i32m i) = Some (VAL_ref_func a) ->
         List.nth_error s.(s_funcs) a = Some cl ->
         List.nth_error f.(f_inst).(inst_types) y <> Some (cl_type cl) ->
-        reduce hs s f [::$VA (VAL_int32 i); AI_basic (BI_call_indirect x y)] hs s f [::AI_trap]
+        reduce hs s f [::$VN (VAL_int32 i); AI_basic (BI_call_indirect x y)] hs s f [::AI_trap]
   | r_call_indirect_failure2 :
       forall s f x (y: typeidx) a i hs,
         stab_elem s f.(f_inst) x (Wasm_int.N_of_uint i32m i) = Some (VAL_ref_func a) ->
         List.nth_error s.(s_funcs) a = None ->
-        reduce hs s f [::$VA (VAL_int32 i); AI_basic (BI_call_indirect x y)] hs s f [::AI_trap]
+        reduce hs s f [::$VN (VAL_int32 i); AI_basic (BI_call_indirect x y)] hs s f [::AI_trap]
   | r_call_indirect_failure3 :
       forall s f x (y: typeidx) i hs,
         stab_elem s f.(f_inst) x (Wasm_int.N_of_uint i32m i) = None ->
-        reduce hs s f [::$VA (VAL_int32 i); AI_basic (BI_call_indirect x y)] hs s f [::AI_trap]
+        reduce hs s f [::$VN (VAL_int32 i); AI_basic (BI_call_indirect x y)] hs s f [::AI_trap]
   | r_call_indirect_failure4 :
       forall s f x (y: typeidx) i hs t,
         stab_elem s f.(f_inst) x (Wasm_int.N_of_uint i32m i) = Some (VAL_ref_null t) ->
-        reduce hs s f [::$VA (VAL_int32 i); AI_basic (BI_call_indirect x y)] hs s f [::AI_trap]
+        reduce hs s f [::$VN (VAL_int32 i); AI_basic (BI_call_indirect x y)] hs s f [::AI_trap]
   | r_invoke_native :
       forall addr cl ts1 ts2 code x ts es ves vs n m k defaults s f inst hs,
         lookup_N s.(s_funcs) addr = Some cl ->
@@ -260,50 +263,50 @@ Inductive reduce : host_state -> store_record -> frame -> list administrative_in
 | r_table_get_success :
   forall x i tabv s f hs,
     stab_elem s f.(f_inst) x (Wasm_int.N_of_uint i32m i) = Some tabv ->
-    reduce hs s f [::$VA (VAL_int32 i); AI_basic (BI_table_get x)] hs s f [::v_to_e (VAL_ref tabv)]
+    reduce hs s f [::$VN (VAL_int32 i); AI_basic (BI_table_get x)] hs s f [::v_to_e (VAL_ref tabv)]
 | r_table_get_failure :
   forall x i s f hs,
     stab_elem s f.(f_inst) x (Wasm_int.N_of_uint i32m i) = None ->
-    reduce hs s f [::$VA (VAL_int32 i); AI_basic (BI_table_get x)] hs s f [::AI_trap]
+    reduce hs s f [::$VN (VAL_int32 i); AI_basic (BI_table_get x)] hs s f [::AI_trap]
 | r_table_set_success :
   forall x i tabv s s' f hs,
     stab_update s f.(f_inst) x (Wasm_int.N_of_uint i32m i) tabv = Some s' ->
-    reduce hs s f [::$VA (VAL_int32 i); v_to_e (VAL_ref tabv); AI_basic (BI_table_set x)] hs s' f [::]
+    reduce hs s f [::$VN (VAL_int32 i); v_to_e (VAL_ref tabv); AI_basic (BI_table_set x)] hs s' f [::]
 | r_table_set_failure :
   forall x i tabv s s' f hs,
     stab_update s f.(f_inst) x (Wasm_int.N_of_uint i32m i) tabv = None ->
-    reduce hs s f [::$VA (VAL_int32 i); v_to_e (VAL_ref tabv); AI_basic (BI_table_set x)] hs s' f [::]
+    reduce hs s f [::$VN (VAL_int32 i); v_to_e (VAL_ref tabv); AI_basic (BI_table_set x)] hs s' f [::]
 | r_table_size :
   forall x a tab sz s s' f hs,
     lookup_N f.(f_inst).(inst_tables) x = Some a ->
     lookup_N s.(s_tables) a = Some tab ->
     tab_size tab = sz ->
-    reduce hs s f [:: AI_basic (BI_table_size x)] hs s' f [::$VA (VAL_int32 (Wasm_int.int_of_Z i32m (Z.of_nat sz)))]
+    reduce hs s f [:: AI_basic (BI_table_size x)] hs s' f [::$VN (VAL_int32 (Wasm_int.int_of_Z i32m (Z.of_nat sz)))]
 | r_table_grow_success :
   forall x n tab sz tabinit s s' f hs,
     stab s f.(f_inst) x = Some tab ->
     tab_size tab = sz ->
     stab_grow s f.(f_inst) x (Wasm_int.N_of_uint i32m n) tabinit = Some s' ->
-    reduce hs s f [::v_to_e (VAL_ref tabinit); $VA (VAL_int32 n); AI_basic (BI_table_set x)]
-      hs s' f [::$VA (VAL_int32 (Wasm_int.int_of_Z i32m (Z.of_nat sz)))]
+    reduce hs s f [::v_to_e (VAL_ref tabinit); $VN (VAL_int32 n); AI_basic (BI_table_set x)]
+      hs s' f [::$VN (VAL_int32 (Wasm_int.int_of_Z i32m (Z.of_nat sz)))]
 | r_table_grow_failure :
   forall x n tab sz tabinit s s' f hs,
     stab s f.(f_inst) x = Some tab ->
     tab_size tab = sz ->
-    reduce hs s f [::v_to_e (VAL_ref tabinit); $VA (VAL_int32 n); AI_basic (BI_table_set x)]
-      hs s' f [::$VA (VAL_int32 int32_minus_one)]
+    reduce hs s f [::v_to_e (VAL_ref tabinit); $VN (VAL_int32 n); AI_basic (BI_table_set x)]
+      hs s' f [::$VN (VAL_int32 int32_minus_one)]
 | r_table_fill_bound :
   forall x i n tab tabv s s' f hs,
     stab s f.(f_inst) x = Some tab ->
     (Wasm_int.N_of_uint i32m i) + (Wasm_int.N_of_uint i32m n) > tab_size tab ->
-    reduce hs s f [::$VA (VAL_int32 i); v_to_e (VAL_ref tabv); $VA (VAL_int32 n); AI_basic (BI_table_fill x)]
+    reduce hs s f [::$VN (VAL_int32 i); v_to_e (VAL_ref tabv); $VN (VAL_int32 n); AI_basic (BI_table_fill x)]
       hs s' f [::AI_trap]
 | r_table_fill_return :
   forall x i n tab tabv s f hs,
     stab s f.(f_inst) x = Some tab ->
     (Wasm_int.N_of_uint i32m i) + (Wasm_int.N_of_uint i32m n) <= tab_size tab ->
     n = Wasm_int.int_zero i32m ->
-    reduce hs s f [::$VA (VAL_int32 i); v_to_e (VAL_ref tabv); $VA (VAL_int32 n); AI_basic (BI_table_fill x)]
+    reduce hs s f [::$VN (VAL_int32 i); v_to_e (VAL_ref tabv); $VN (VAL_int32 n); AI_basic (BI_table_fill x)]
       hs s f [::]
 | r_table_fill_step :
   forall x i n tab tabv n' i' s f hs,
@@ -312,16 +315,16 @@ Inductive reduce : host_state -> store_record -> frame -> list administrative_in
     n <> Wasm_int.int_zero i32m ->
     Wasm_int.N_of_uint i32m n' = N.sub (Wasm_int.N_of_uint i32m n) 1 ->
     Wasm_int.N_of_uint i32m i' = N.add (Wasm_int.N_of_uint i32m i) 1 ->
-    reduce hs s f [::$VA (VAL_int32 i); v_to_e (VAL_ref tabv); $VA (VAL_int32 n); AI_basic (BI_table_fill x)]
-      hs s f [::$VA (VAL_int32 i); v_to_e (VAL_ref tabv); AI_basic (BI_table_set x);
-              $VA (VAL_int32 i'); v_to_e (VAL_ref tabv); $VA (VAL_int32 n'); AI_basic (BI_table_fill x)]
+    reduce hs s f [::$VN (VAL_int32 i); v_to_e (VAL_ref tabv); $VN (VAL_int32 n); AI_basic (BI_table_fill x)]
+      hs s f [::$VN (VAL_int32 i); v_to_e (VAL_ref tabv); AI_basic (BI_table_set x);
+              $VN (VAL_int32 i'); v_to_e (VAL_ref tabv); $VN (VAL_int32 n'); AI_basic (BI_table_fill x)]
 | r_table_copy_bound :
   forall x y src dst n tabx taby s f hs,
     stab s f.(f_inst) x = Some tabx ->
     stab s f.(f_inst) y = Some taby ->
     (((Wasm_int.N_of_uint i32m src) + (Wasm_int.N_of_uint i32m n) > tab_size taby) \/
        ((Wasm_int.N_of_uint i32m dst) + (Wasm_int.N_of_uint i32m n) > tab_size tabx)) ->
-    reduce hs s f [::$VA (VAL_int32 dst); $VA (VAL_int32 src); $VA (VAL_int32 n); AI_basic (BI_table_copy x y)]
+    reduce hs s f [::$VN (VAL_int32 dst); $VN (VAL_int32 src); $VN (VAL_int32 n); AI_basic (BI_table_copy x y)]
       hs s f [::AI_trap]
 | r_table_copy_return :
   forall x y src dst n tabx taby s f hs,
@@ -330,7 +333,7 @@ Inductive reduce : host_state -> store_record -> frame -> list administrative_in
     ((Wasm_int.N_of_uint i32m src) + (Wasm_int.N_of_uint i32m n) <= tab_size taby) ->
     ((Wasm_int.N_of_uint i32m dst) + (Wasm_int.N_of_uint i32m n) <= tab_size tabx) ->
     n = Wasm_int.int_zero i32m ->
-    reduce hs s f [::$VA (VAL_int32 dst); $VA (VAL_int32 src); $VA (VAL_int32 n); AI_basic (BI_table_copy x y)]
+    reduce hs s f [::$VN (VAL_int32 dst); $VN (VAL_int32 src); $VN (VAL_int32 n); AI_basic (BI_table_copy x y)]
       hs s f [::]
 | r_table_copy_forward :
   forall x y src dst n tabx taby src' dst' n' s f hs,
@@ -343,9 +346,9 @@ Inductive reduce : host_state -> store_record -> frame -> list administrative_in
     Wasm_int.N_of_uint i32m n' = N.sub (Wasm_int.N_of_uint i32m n) 1 ->
     Wasm_int.N_of_uint i32m src' = N.add (Wasm_int.N_of_uint i32m src) 1 ->
     Wasm_int.N_of_uint i32m dst' = N.add (Wasm_int.N_of_uint i32m dst) 1 ->
-    reduce hs s f [::$VA (VAL_int32 dst); $VA (VAL_int32 src); $VA (VAL_int32 n); AI_basic (BI_table_copy x y)]
-      hs s f [:: $VA (VAL_int32 dst); $VA (VAL_int32 src); AI_basic (BI_table_get y); AI_basic (BI_table_set x);
-              $VA (VAL_int32 dst'); $VA (VAL_int32 src'); $VA (VAL_int32 n'); AI_basic (BI_table_copy x y)]
+    reduce hs s f [::$VN (VAL_int32 dst); $VN (VAL_int32 src); $VN (VAL_int32 n); AI_basic (BI_table_copy x y)]
+      hs s f [:: $VN (VAL_int32 dst); $VN (VAL_int32 src); AI_basic (BI_table_get y); AI_basic (BI_table_set x);
+              $VN (VAL_int32 dst'); $VN (VAL_int32 src'); $VN (VAL_int32 n'); AI_basic (BI_table_copy x y)]
 | r_table_copy_backward :
   forall x y src dst n tabx taby src' dst' n' s f hs,
     stab s f.(f_inst) x = Some tabx ->
@@ -357,16 +360,16 @@ Inductive reduce : host_state -> store_record -> frame -> list administrative_in
     Wasm_int.N_of_uint i32m n' = N.add (Wasm_int.N_of_uint i32m n) 1 ->
     Wasm_int.N_of_uint i32m src' = N.sub (Wasm_int.N_of_uint i32m src + Wasm_int.N_of_uint i32m n) 1 ->
     Wasm_int.N_of_uint i32m dst' = N.sub (Wasm_int.N_of_uint i32m dst + Wasm_int.N_of_uint i32m n) 1 ->
-    reduce hs s f [::$VA (VAL_int32 dst); $VA (VAL_int32 src); $VA (VAL_int32 n); AI_basic (BI_table_copy x y)]
-      hs s f [:: $VA (VAL_int32 dst'); $VA (VAL_int32 src'); AI_basic (BI_table_get y); AI_basic (BI_table_set x);
-              $VA (VAL_int32 dst); $VA (VAL_int32 src); $VA (VAL_int32 n'); AI_basic (BI_table_copy x y)]
+    reduce hs s f [::$VN (VAL_int32 dst); $VN (VAL_int32 src); $VN (VAL_int32 n); AI_basic (BI_table_copy x y)]
+      hs s f [:: $VN (VAL_int32 dst'); $VN (VAL_int32 src'); AI_basic (BI_table_get y); AI_basic (BI_table_set x);
+              $VN (VAL_int32 dst); $VN (VAL_int32 src); $VN (VAL_int32 n'); AI_basic (BI_table_copy x y)]
 | r_table_init_bound :
   forall x y src dst n tab elem s f hs,
     stab s f.(f_inst) x = Some tab ->
     selem s f.(f_inst) y = Some elem ->
     (((Wasm_int.N_of_uint i32m src) + (Wasm_int.N_of_uint i32m n) > elem_size elem) \/
        ((Wasm_int.N_of_uint i32m dst) + (Wasm_int.N_of_uint i32m n) > tab_size tab)) ->
-    reduce hs s f [::$VA (VAL_int32 dst); $VA (VAL_int32 src); $VA (VAL_int32 n); AI_basic (BI_table_init x y)]
+    reduce hs s f [::$VN (VAL_int32 dst); $VN (VAL_int32 src); $VN (VAL_int32 n); AI_basic (BI_table_init x y)]
       hs s f [::AI_trap]
 | r_table_init_return :
   forall x y src dst n tab elem s f hs,
@@ -375,7 +378,7 @@ Inductive reduce : host_state -> store_record -> frame -> list administrative_in
     ((Wasm_int.N_of_uint i32m src) + (Wasm_int.N_of_uint i32m n) <= elem_size elem) ->
     ((Wasm_int.N_of_uint i32m dst) + (Wasm_int.N_of_uint i32m n) <= tab_size tab) ->
     n = Wasm_int.int_zero i32m ->
-    reduce hs s f [::$VA (VAL_int32 dst); $VA (VAL_int32 src); $VA (VAL_int32 n); AI_basic (BI_table_init x y)]
+    reduce hs s f [::$VN (VAL_int32 dst); $VN (VAL_int32 src); $VN (VAL_int32 n); AI_basic (BI_table_init x y)]
       hs s f [::]
 | r_table_init_step :
   forall x y src dst n tab elem src' dst' n' v s f hs,
@@ -388,9 +391,9 @@ Inductive reduce : host_state -> store_record -> frame -> list administrative_in
     Wasm_int.N_of_uint i32m n' = N.sub (Wasm_int.N_of_uint i32m n) 1 ->
     Wasm_int.N_of_uint i32m src' = N.add (Wasm_int.N_of_uint i32m src) 1 ->
     Wasm_int.N_of_uint i32m dst' = N.add (Wasm_int.N_of_uint i32m dst) 1 ->
-    reduce hs s f [::$VA (VAL_int32 dst); $VA (VAL_int32 src); $VA (VAL_int32 n); AI_basic (BI_table_init x y)]
-      hs s f [:: $VA (VAL_int32 dst); v_to_e (VAL_ref v); AI_basic (BI_table_set x);
-              $VA (VAL_int32 dst'); $VA (VAL_int32 src'); $VA (VAL_int32 n'); AI_basic (BI_table_init x y)]
+    reduce hs s f [::$VN (VAL_int32 dst); $VN (VAL_int32 src); $VN (VAL_int32 n); AI_basic (BI_table_init x y)]
+      hs s f [:: $VN (VAL_int32 dst); v_to_e (VAL_ref v); AI_basic (BI_table_set x);
+              $VN (VAL_int32 dst'); $VN (VAL_int32 src'); $VN (VAL_int32 n'); AI_basic (BI_table_init x y)]
 | r_elem_drop:
   forall x hs s f s',
     selem_drop s f.(f_inst) x = Some s' ->
@@ -402,84 +405,84 @@ Inductive reduce : host_state -> store_record -> frame -> list administrative_in
     smem_ind s f.(f_inst) = Some i ->
     lookup_N s.(s_mems) i = Some m ->
     load m (Wasm_int.N_of_uint i32m k) off (tnum_length t) = Some bs ->
-    reduce hs s f [::$VA (VAL_int32 k); AI_basic (BI_load t None a off)] hs s f [::$VA (wasm_deserialise bs t)]
+    reduce hs s f [::$VN (VAL_int32 k); AI_basic (BI_load t None a off)] hs s f [::$VN (wasm_deserialise bs t)]
 | r_load_failure :
   forall s i f t k a off m hs,
     smem_ind s f.(f_inst) = Some i ->
     lookup_N s.(s_mems) i = Some m ->
     load m (Wasm_int.N_of_uint i32m k) off (tnum_length t) = None ->
-    reduce hs s f [::$VA (VAL_int32 k); AI_basic (BI_load t None a off)] hs s f [::AI_trap]
+    reduce hs s f [::$VN (VAL_int32 k); AI_basic (BI_load t None a off)] hs s f [::AI_trap]
 | r_load_packed_success :
   forall s i f t tp k a off m bs sx hs,
     smem_ind s f.(f_inst) = Some i ->
     lookup_N s.(s_mems) i = Some m ->
     load_packed sx m (Wasm_int.N_of_uint i32m k) off (tp_length tp) (tnum_length t) = Some bs ->
-    reduce hs s f [::$VA (VAL_int32 k); AI_basic (BI_load t (Some (tp, sx)) a off)] hs s f [::$VA (wasm_deserialise bs t)]
+    reduce hs s f [::$VN (VAL_int32 k); AI_basic (BI_load t (Some (tp, sx)) a off)] hs s f [::$VN (wasm_deserialise bs t)]
 | r_load_packed_failure :
   forall s i f t tp k a off m sx hs,
     smem_ind s f.(f_inst) = Some i ->
     lookup_N s.(s_mems) i = Some m ->
     load_packed sx m (Wasm_int.N_of_uint i32m k) off (tp_length tp) (tnum_length t) = None ->
-    reduce hs s f [::$VA (VAL_int32 k); AI_basic (BI_load t (Some (tp, sx)) a off)] hs s f [::AI_trap]
+    reduce hs s f [::$VN (VAL_int32 k); AI_basic (BI_load t (Some (tp, sx)) a off)] hs s f [::AI_trap]
 | r_store_success :
   forall t v s i f mem' k a off m hs,
     typeof_num v = t ->
     smem_ind s f.(f_inst) = Some i ->
     lookup_N s.(s_mems) i = Some m ->
     store m (Wasm_int.N_of_uint i32m k) off (bits v) (tnum_length t) = Some mem' ->
-    reduce hs s f [::$VA (VAL_int32 k); $VA v; AI_basic (BI_store t None a off)] hs (upd_s_mem s (set_nth mem' s.(s_mems) i mem')) f [::]
+    reduce hs s f [::$VN (VAL_int32 k); $VN v; AI_basic (BI_store t None a off)] hs (upd_s_mem s (set_nth mem' s.(s_mems) i mem')) f [::]
 | r_store_failure :
   forall t v s i f m k off a hs,
     typeof_num v = t ->
     smem_ind s f.(f_inst) = Some i ->
     lookup_N s.(s_mems) i = Some m ->
     store m (Wasm_int.N_of_uint i32m k) off (bits v) (tnum_length t) = None ->
-    reduce hs s f [::$VA (VAL_int32 k); $VA v; AI_basic (BI_store t None a off)] hs s f [::AI_trap]
+    reduce hs s f [::$VN (VAL_int32 k); $VN v; AI_basic (BI_store t None a off)] hs s f [::AI_trap]
 | r_store_packed_success :
   forall t v s i f m k off a mem' tp hs,
     typeof_num v = t ->
     smem_ind s f.(f_inst) = Some i ->
     lookup_N s.(s_mems) i = Some m ->
     store_packed m (Wasm_int.N_of_uint i32m k) off (bits v) (tp_length tp) = Some mem' ->
-    reduce hs s f [::$VA (VAL_int32 k); $VA v; AI_basic (BI_store t (Some tp) a off)] hs (upd_s_mem s (set_nth mem' s.(s_mems) i mem')) f [::]
+    reduce hs s f [::$VN (VAL_int32 k); $VN v; AI_basic (BI_store t (Some tp) a off)] hs (upd_s_mem s (set_nth mem' s.(s_mems) i mem')) f [::]
 | r_store_packed_failure :
   forall t v s i f m k off a tp hs,
     typeof_num v = t ->
     smem_ind s f.(f_inst) = Some i ->
     lookup_N s.(s_mems) i = Some m ->
     store_packed m (Wasm_int.N_of_uint i32m k) off (bits v) (tp_length tp) = None ->
-    reduce hs s f [::$VA (VAL_int32 k); $VA v; AI_basic (BI_store t (Some tp) a off)] hs s f [::AI_trap]
+    reduce hs s f [::$VN (VAL_int32 k); $VN v; AI_basic (BI_store t (Some tp) a off)] hs s f [::AI_trap]
 | r_memory_size :
   forall i f m n s hs,
     smem_ind s f.(f_inst) = Some i ->
     lookup_N s.(s_mems) i = Some m ->
     mem_size m = n ->
-    reduce hs s f [::AI_basic (BI_memory_size)] hs s f [::$VA (VAL_int32 (Wasm_int.int_of_Z i32m (Z.of_nat n)))]
+    reduce hs s f [::AI_basic (BI_memory_size)] hs s f [::$VN (VAL_int32 (Wasm_int.int_of_Z i32m (Z.of_nat n)))]
 | r_memory_grow_success :
   forall s i f m n mem' c hs,
     smem_ind s f.(f_inst) = Some i ->
     lookup_N s.(s_mems) i = Some m ->
     mem_size m = n ->
     mem_grow m (Wasm_int.N_of_uint i32m c) = Some mem' ->
-    reduce hs s f [::$VA (VAL_int32 c); AI_basic BI_memory_grow] hs (upd_s_mem s (set_nth mem' s.(s_mems) i mem')) f [::$VA (VAL_int32 (Wasm_int.int_of_Z i32m (Z.of_nat n)))]
+    reduce hs s f [::$VN (VAL_int32 c); AI_basic BI_memory_grow] hs (upd_s_mem s (set_nth mem' s.(s_mems) i mem')) f [::$VN (VAL_int32 (Wasm_int.int_of_Z i32m (Z.of_nat n)))]
 | r_memory_grow_failure :
   forall i f m n s c hs,
     smem_ind s f.(f_inst) = Some i ->
     lookup_N s.(s_mems) i = Some m ->
     mem_size m = n ->
-    reduce hs s f [::$VA (VAL_int32 c); AI_basic BI_memory_grow] hs s f [::$VA (VAL_int32 int32_minus_one)]
+    reduce hs s f [::$VN (VAL_int32 c); AI_basic BI_memory_grow] hs s f [::$VN (VAL_int32 int32_minus_one)]
 | r_memory_fill_bound:
   forall s f mem d n v hs,
     smem s f.(f_inst) = Some mem ->
     (Wasm_int.N_of_uint i32m d) + (Wasm_int.N_of_uint i32m n) > mem_length mem ->
-    reduce hs s f [::$VA (VAL_int32 d); $VA (VAL_int32 v); $VA (VAL_int32 n); AI_basic (BI_memory_fill)]
+    reduce hs s f [::$VN (VAL_int32 d); $VN (VAL_int32 v); $VN (VAL_int32 n); AI_basic (BI_memory_fill)]
            hs s f [::AI_trap]
 | r_memory_fill_return:
   forall s f mem d n v hs,
     smem s f.(f_inst) = Some mem ->
     (Wasm_int.N_of_uint i32m d) + (Wasm_int.N_of_uint i32m n) <= mem_length mem ->
     n = Wasm_int.int_zero i32m ->
-    reduce hs s f [::$VA (VAL_int32 d); $VA (VAL_int32 v); $VA (VAL_int32 n); AI_basic (BI_memory_fill)]
+    reduce hs s f [::$VN (VAL_int32 d); $VN (VAL_int32 v); $VN (VAL_int32 n); AI_basic (BI_memory_fill)]
            hs s f [::]
 | r_memory_fill_step:
   forall s f mem d n d' n' v hs,
@@ -488,15 +491,15 @@ Inductive reduce : host_state -> store_record -> frame -> list administrative_in
     n <> Wasm_int.int_zero i32m ->
     Wasm_int.N_of_uint i32m n' = N.sub (Wasm_int.N_of_uint i32m n) 1 ->
     Wasm_int.N_of_uint i32m d' = N.add (Wasm_int.N_of_uint i32m d) 1 ->
-    reduce hs s f [::$VA (VAL_int32 d); $VA (VAL_int32 v); $VA (VAL_int32 n); AI_basic (BI_memory_fill)]
-      hs s f [::$VA (VAL_int32 d); $VA (VAL_int32 v); AI_basic (BI_store T_i32 (Some Tp_i8) N0 N0);
-                $VA (VAL_int32 d'); $VA (VAL_int32 v); $VA (VAL_int32 n'); AI_basic (BI_memory_fill)]
+    reduce hs s f [::$VN (VAL_int32 d); $VN (VAL_int32 v); $VN (VAL_int32 n); AI_basic (BI_memory_fill)]
+      hs s f [::$VN (VAL_int32 d); $VN (VAL_int32 v); AI_basic (BI_store T_i32 (Some Tp_i8) N0 N0);
+                $VN (VAL_int32 d'); $VN (VAL_int32 v); $VN (VAL_int32 n'); AI_basic (BI_memory_fill)]
 | r_memory_copy_bound :
   forall src dst n mem s f hs,
     smem s f.(f_inst) = Some mem ->
     (((Wasm_int.N_of_uint i32m src) + (Wasm_int.N_of_uint i32m n) > mem_length mem) \/
        ((Wasm_int.N_of_uint i32m dst) + (Wasm_int.N_of_uint i32m n) > mem_length mem)) ->
-    reduce hs s f [::$VA (VAL_int32 dst); $VA (VAL_int32 src); $VA (VAL_int32 n); AI_basic (BI_memory_copy)]
+    reduce hs s f [::$VN (VAL_int32 dst); $VN (VAL_int32 src); $VN (VAL_int32 n); AI_basic (BI_memory_copy)]
       hs s f [::AI_trap]
 | r_memory_copy_return :
   forall src dst n mem s f hs,
@@ -504,7 +507,7 @@ Inductive reduce : host_state -> store_record -> frame -> list administrative_in
     ((Wasm_int.N_of_uint i32m src) + (Wasm_int.N_of_uint i32m n) <= mem_length mem) ->
     ((Wasm_int.N_of_uint i32m dst) + (Wasm_int.N_of_uint i32m n) <= mem_length mem) ->
     n = Wasm_int.int_zero i32m ->
-    reduce hs s f [::$VA (VAL_int32 dst); $VA (VAL_int32 src); $VA (VAL_int32 n); AI_basic (BI_memory_copy)]
+    reduce hs s f [::$VN (VAL_int32 dst); $VN (VAL_int32 src); $VN (VAL_int32 n); AI_basic (BI_memory_copy)]
       hs s f [::]
 | r_memory_copy_forward :
   forall src dst n mem src' dst' n' s f hs,
@@ -516,9 +519,9 @@ Inductive reduce : host_state -> store_record -> frame -> list administrative_in
     Wasm_int.N_of_uint i32m n' = N.sub (Wasm_int.N_of_uint i32m n) 1 ->
     Wasm_int.N_of_uint i32m src' = N.add (Wasm_int.N_of_uint i32m src) 1 ->
     Wasm_int.N_of_uint i32m dst' = N.add (Wasm_int.N_of_uint i32m dst) 1 ->
-    reduce hs s f [::$VA (VAL_int32 dst); $VA (VAL_int32 src); $VA (VAL_int32 n); AI_basic (BI_memory_copy)]
-      hs s f [:: $VA (VAL_int32 dst); $VA (VAL_int32 src); AI_basic (BI_load T_i32 (Some (Tp_i8, SX_U)) N0 N0); AI_basic (BI_store T_i32 (Some (Tp_i8)) N0 N0);
-              $VA (VAL_int32 dst'); $VA (VAL_int32 src'); $VA (VAL_int32 n'); AI_basic (BI_memory_copy)]
+    reduce hs s f [::$VN (VAL_int32 dst); $VN (VAL_int32 src); $VN (VAL_int32 n); AI_basic (BI_memory_copy)]
+      hs s f [:: $VN (VAL_int32 dst); $VN (VAL_int32 src); AI_basic (BI_load T_i32 (Some (Tp_i8, SX_U)) N0 N0); AI_basic (BI_store T_i32 (Some (Tp_i8)) N0 N0);
+              $VN (VAL_int32 dst'); $VN (VAL_int32 src'); $VN (VAL_int32 n'); AI_basic (BI_memory_copy)]
 | r_memory_copy_backward :
   forall src dst n mem src' dst' n' s f hs,
     smem s f.(f_inst) = Some mem ->
@@ -529,16 +532,16 @@ Inductive reduce : host_state -> store_record -> frame -> list administrative_in
     Wasm_int.N_of_uint i32m n' = N.add (Wasm_int.N_of_uint i32m n) 1 ->
     Wasm_int.N_of_uint i32m src' = N.sub (Wasm_int.N_of_uint i32m src + Wasm_int.N_of_uint i32m n) 1 ->
     Wasm_int.N_of_uint i32m dst' = N.sub (Wasm_int.N_of_uint i32m dst + Wasm_int.N_of_uint i32m n) 1 ->
-    reduce hs s f [::$VA (VAL_int32 dst); $VA (VAL_int32 src); $VA (VAL_int32 n); AI_basic (BI_memory_copy)]
-      hs s f [:: $VA (VAL_int32 dst'); $VA (VAL_int32 src'); AI_basic (BI_load T_i32 (Some (Tp_i8, SX_U)) N0 N0); AI_basic (BI_store T_i32 (Some (Tp_i8)) N0 N0);
-              $VA (VAL_int32 dst); $VA (VAL_int32 src); $VA (VAL_int32 n'); AI_basic (BI_memory_copy)]
+    reduce hs s f [::$VN (VAL_int32 dst); $VN (VAL_int32 src); $VN (VAL_int32 n); AI_basic (BI_memory_copy)]
+      hs s f [:: $VN (VAL_int32 dst'); $VN (VAL_int32 src'); AI_basic (BI_load T_i32 (Some (Tp_i8, SX_U)) N0 N0); AI_basic (BI_store T_i32 (Some (Tp_i8)) N0 N0);
+              $VN (VAL_int32 dst); $VN (VAL_int32 src); $VN (VAL_int32 n'); AI_basic (BI_memory_copy)]
 | r_memory_init_bound :
   forall x src dst n mem data s f hs,
     smem s f.(f_inst) = Some mem ->
     sdata s f.(f_inst) x = Some data ->
     (((Wasm_int.N_of_uint i32m src) + (Wasm_int.N_of_uint i32m n) > data_size data) \/
        ((Wasm_int.N_of_uint i32m dst) + (Wasm_int.N_of_uint i32m n) > mem_length mem)) ->
-    reduce hs s f [::$VA (VAL_int32 dst); $VA (VAL_int32 src); $VA (VAL_int32 n); AI_basic (BI_memory_init x)]
+    reduce hs s f [::$VN (VAL_int32 dst); $VN (VAL_int32 src); $VN (VAL_int32 n); AI_basic (BI_memory_init x)]
       hs s f [::AI_trap]
 | r_memory_init_return :
   forall x src dst n mem data s f hs,
@@ -547,7 +550,7 @@ Inductive reduce : host_state -> store_record -> frame -> list administrative_in
     ((Wasm_int.N_of_uint i32m src) + (Wasm_int.N_of_uint i32m n) <= data_size data) ->
     ((Wasm_int.N_of_uint i32m dst) + (Wasm_int.N_of_uint i32m n) <= mem_length mem) ->
     n = Wasm_int.int_zero i32m ->
-    reduce hs s f [::$VA (VAL_int32 dst); $VA (VAL_int32 src); $VA (VAL_int32 n); AI_basic (BI_memory_init x)]
+    reduce hs s f [::$VN (VAL_int32 dst); $VN (VAL_int32 src); $VN (VAL_int32 n); AI_basic (BI_memory_init x)]
       hs s f [::]
 | r_memory_init_step :
   forall x src dst n mem data src' dst' n' b s f hs,
@@ -560,23 +563,23 @@ Inductive reduce : host_state -> store_record -> frame -> list administrative_in
     Wasm_int.N_of_uint i32m n' = N.sub (Wasm_int.N_of_uint i32m n) 1 ->
     Wasm_int.N_of_uint i32m src' = N.add (Wasm_int.N_of_uint i32m src) 1 ->
     Wasm_int.N_of_uint i32m dst' = N.add (Wasm_int.N_of_uint i32m dst) 1 ->
-    reduce hs s f [::$VA (VAL_int32 dst); $VA (VAL_int32 src); $VA (VAL_int32 n); AI_basic (BI_memory_init x)]
-      hs s f [:: $VA (VAL_int32 dst); v_to_e (VAL_num (wasm_deserialise [::b] T_i32)); AI_basic (BI_store T_i32 (Some Tp_i8) N0 N0);
-              $VA (VAL_int32 dst'); $VA (VAL_int32 src'); $VA (VAL_int32 n'); AI_basic (BI_memory_init x)]
+    reduce hs s f [::$VN (VAL_int32 dst); $VN (VAL_int32 src); $VN (VAL_int32 n); AI_basic (BI_memory_init x)]
+      hs s f [:: $VN (VAL_int32 dst); v_to_e (VAL_num (wasm_deserialise [::b] T_i32)); AI_basic (BI_store T_i32 (Some Tp_i8) N0 N0);
+              $VN (VAL_int32 dst'); $VN (VAL_int32 src'); $VN (VAL_int32 n'); AI_basic (BI_memory_init x)]
 | r_data_drop:
   forall x hs s f s',
     sdata_drop s f.(f_inst) x = Some s' ->
     reduce hs s f [::AI_basic (BI_data_drop x)] hs s' f [::]
 
                
-  (** label and local **)
+  (** label and frame **)
   | r_label :
       forall s f es les s' f' es' les' k (lh: lholed k) hs hs',
         reduce hs s f es hs' s' f' es' ->
         lfill lh es = les ->
         lfill lh es' = les' ->
         reduce hs s f les hs' s' f' les'
-  | r_local :
+  | r_frame :
       forall s f es s' f' es' n f0 hs hs',
         reduce hs s f es hs' s' f' es' ->
         reduce hs s f0 [::AI_frame n f es] hs' s' f0 [::AI_frame n f' es']
